src/automata/epsnfa_append.lean
@@ -1,0 +1,97 @@
+import data.set.basic
+import data.set.finite
+import automata.epsnfa
+import languages.basic
+
+open set epsnfa languages
+
+namespace epsnfa
+
+variables {S Q Q1 Q2 : Type}
+
+inductive U (Q1 Q2 : Type) : Type
+| left (q : Q1) : U
+| right (q : Q2) : U
+
+def epsnfa_append (e1 : epsNFA S Q1) (e2 : epsNFA S Q2) : epsNFA S (U Q1 Q2) := {
+    start := U.left e1.start,
+    term := U.right e2.term,
+    next := λ q c, begin
+        cases q, 
+        { exact U.left '' (e1.next q c) },
+        { exact U.right '' (e2.next q c) }, 
+    end,
+    eps := λ q, begin
+        cases q, {
+            by_cases q = e1.term,
+            exact (U.left '' (e1.eps q)) ∪ {U.right e2.start},
+            exact (U.left '' (e1.eps q)),
+        }, { 
+            exact U.right '' e2.eps q,
+        },
+    end
+}
+
+lemma epsnfa_append_go_left {e1 : epsNFA S Q1} {e2 : epsNFA S Q2} 
+    {a b : Q1} {w : list S} 
+    :  go e1 a w b ↔ go (epsnfa_append e1 e2) (U.left a) w (U.left b) :=
+begin
+    split, {
+        sorry,
+    }, {
+        sorry,
+    }
+end 
+
+lemma epsnfa_append_go_right {e1 : epsNFA S Q1} {e2 : epsNFA S Q2} 
+    {a b : Q2} {w : list S}
+    : go e2 a w b ↔ go (epsnfa_append e1 e2) (U.right a) w (U.right b) :=
+begin
+    split, {
+        intro goright,
+        induction goright, {
+            exact go.finish,
+        }, {
+            refine go.step _ goright_ih,
+            dsimp [epsnfa_append],
+            simpa only [mem_image, exists_eq_right], 
+        }, {
+            refine go.eps _ goright_ih,
+            dsimp [epsnfa_append],
+            simpa only [mem_image, exists_eq_right],
+        }
+    }, {
+        intro goappend,
+        generalize ha : (U.right : Q2 → @U Q1 Q2) a = ua,
+        generalize hb : (U.right : Q2 → @U Q1 Q2) b = ub,
+        rw [ha, hb] at goappend,
+        induction goappend generalizing a, {
+            subst hb,
+            injection ha with ha,
+            subst ha,
+            exact go.finish,
+        }, {
+            sorry,
+        }, {
+            sorry,
+        }
+    }
+end 
+
+
+theorem epsnfa_union_correct (e1 : epsNFA S Q1) (e2 : epsNFA S Q2):
+    lang_of_epsnfa e1 * lang_of_epsnfa e2 = lang_of_epsnfa (epsnfa_append e1 e2) :=
+begin
+    apply subset.antisymm, {
+        rintro _ ⟨left, right, hleft, hright, rfl⟩,
+        dsimp at hleft hright,
+        apply epsnfa_go_trans (epsnfa_append_go_left.1 hleft),
+        refine @go.eps _ _ _ _ _ (U.right e2.start) _ _ _,
+        simp [epsnfa_append], 
+        exact epsnfa_append_go_right.1 hright,
+    }, {
+        sorry,
+    }
+end
+
+end epsnfa
